hide QUIC.*.Public parsers behind interfaces

src/QUIC.Impl.Public.fst
@@ -1,5 +1,6 @@
 module QUIC.Impl.Public
-include QUIC.Spec.Public
+open QUIC.Spec.Public
+friend QUIC.Spec.Public
 
 module LP = LowParse.Low
 
@@ -28,8 +29,6 @@ let validate_long_handshake_body : LP.validator parse_long_handshake_body =
 inline_for_extraction
 let validate_long_retry_body : LP.validator parse_long_retry_body =
   validate_common_long `LP.validate_nondep_then` LP.validate_bounded_vlbytes 0 20
-
-module U32 = FStar.UInt32
 
 inline_for_extraction
 let validate_long_initial_body : LP.validator parse_long_initial_body =
@@ -94,136 +93,10 @@ let destr_first_byte
 = norm [primops; iota; zeta; delta_attr [`%LPB.filter_bitsum'_t_attr]]
   (LPB.mk_destr_bitsum'_t first_byte)
 
-module S = QUIC.Spec.Public
-module B = LowStar.Buffer
-module U8 = FStar.UInt8
-
-noeq
-type long_header_specifics =
-| PInitial:
-  (payload_and_pn_length: payload_and_pn_length_t) ->
-  (token: B.buffer U8.t) ->
-  (token_length: U32.t { let v = U32.v token_length in v == B.length token /\ 0 <= v /\ v <= token_max_len }) ->
-  long_header_specifics
-| PZeroRTT:
-  (payload_and_pn_length: payload_and_pn_length_t) ->
-  long_header_specifics
-| PHandshake:
-  (payload_and_pn_length: payload_and_pn_length_t) ->
-  long_header_specifics
-| PRetry:
-  odcid: B.buffer U8.t ->
-  odcil: U32.t { let v = U32.v odcil in v = B.length odcid /\ 0 <= v /\ v <= 20 } ->
-  long_header_specifics
-
-noeq
-type header =
-| PLong:
-  (protected_bits: bitfield 4) ->
-  (version: U32.t) ->
-  dcid: B.buffer U8.t ->
-  dcil: U32.t { let v = U32.v dcil in v == B.length dcid /\ 0 <= v /\ v <= 20 } ->
-  scid: B.buffer U8.t ->
-  scil: U32.t { let v = U32.v scil in v == B.length scid /\ 0 <= v /\ v <= 20 } ->
-  (spec: long_header_specifics) ->
-  header
-| PShort:
-  (protected_bits: bitfield 5) ->
-  (spin: bool) ->
-  cid: B.buffer U8.t ->
-  cid_len: U32.t{
-    let l = U32.v cid_len in
-    l == B.length cid /\
-    0 <= l /\ l <= 20
-  } ->
-  header
-
-module HS = FStar.HyperStack
-
-let header_live (h: header) (m: HS.mem) : GTot Type0 =
-  match h with
-  | PShort protected_bits spin cid cid_len ->
-    B.live m cid
-  | PLong protected_bits version dcid dcil scid scil spec ->
-    B.live m dcid /\ B.live m scid /\
-    begin match spec with
-    | PInitial payload_and_pn_length token token_length ->
-      B.live m token
-    | PRetry odcid odcil ->
-      B.live m odcid
-    | _ -> True
-    end
-
-let header_footprint (h: header) : GTot B.loc =
-  match h with
-  | PShort protected_bits spin cid cid_len ->
-    B.loc_buffer cid
-  | PLong protected_bits version dcid dcil scid scil spec ->
-    B.loc_buffer dcid `B.loc_union` B.loc_buffer scid `B.loc_union`
-    begin match spec with
-    | PInitial payload_and_pn_length token token_length ->
-      B.loc_buffer token
-    | PRetry odcid odcil ->
-      B.loc_buffer odcid
-    | _ -> B.loc_none
-    end
-
-let header_live_loc_not_unused_in_footprint (h: header) (m: HS.mem) : Lemma
-  (requires (header_live h m))
-  (ensures (B.loc_not_unused_in m `B.loc_includes` header_footprint h))
-= ()
-
-module FB = FStar.Bytes
-
-let g_header (h: header) (m: HS.mem) : GTot S.header =
-  match h with
-  | PShort protected_bits spin cid cid_len ->
-    S.PShort protected_bits spin (FB.hide (B.as_seq m cid))
-  | PLong protected_bits version dcid dcil scid scil spec ->
-    S.PLong protected_bits version (FB.hide (B.as_seq m dcid)) (FB.hide (B.as_seq m scid))
-    begin match spec with
-    | PInitial payload_and_pn_length token token_length ->
-      S.PInitial (FB.hide (B.as_seq m token)) payload_and_pn_length 
-    | PRetry odcid odcil ->
-      S.PRetry (FB.hide (B.as_seq m odcid))
-    | PHandshake payload_and_pn_length -> S.PHandshake payload_and_pn_length
-    | PZeroRTT payload_and_pn_length -> S.PZeroRTT payload_and_pn_length    
-    end
-
-let frame_header_live
-  (h: header)
-  (l: B.loc)
-  (m1 m2: HS.mem)
-: Lemma
-  (requires (
-    header_live h m1 /\
-    B.modifies l m1 m2 /\
-    B.loc_disjoint l (header_footprint h)
-  ))
-  (ensures (header_live h m2))
-= ()
-
-let frame_header
-  (h: header)
-  (l: B.loc)
-  (m1 m2: HS.mem)
-: Lemma
-  (requires (
-    header_live h m1 /\
-    B.modifies l m1 m2 /\
-    B.loc_disjoint l (header_footprint h)
-  ))
-  (ensures (header_live h m2 /\ g_header h m2 == g_header h m1))
-= ()
-
 
 (* Length computations need to be transparent because the precondition
 to QUIC.Impl.encrypt requires the user to provide a destination buffer
 large enough to contain the byte representation of the header *)
-
-module U64 = FStar.UInt64
-
-module HST = FStar.HyperStack.ST
 
 let read_header_body_post
   (sl: LP.slice (B.trivial_preorder _) (B.trivial_preorder _))
@@ -491,29 +364,6 @@ let read_header_body
     read_header_body_long_handshake sl cid_len protected_bits len
   | (| Long, (| (), (| ZeroRTT, (protected_bits, ()) |) |) |) ->
     read_header_body_long_zero_rtt sl cid_len protected_bits len
-
-val read_header
-  (packet: B.buffer U8.t)
-  (packet_len: U32.t { let v = U32.v packet_len in v == B.length packet })
-  (cid_len: U32.t { U32.v cid_len <= 20 } )
-: HST.Stack (option (header & U32.t))
-  (requires (fun h ->
-    B.live h packet
-  ))
-  (ensures (fun h res h' ->
-    B.modifies B.loc_none h h' /\
-    begin
-      match LP.parse (parse_header cid_len) (B.as_seq h packet), res with
-      | None, None -> True
-      | Some (x, len), Some (x', len') ->
-        header_live x' h' /\
-        len <= B.length packet /\
-        B.loc_buffer (B.gsub packet 0ul (U32.uint_to_t len)) `B.loc_includes` header_footprint x' /\
-        g_header x' h' == x /\
-        U32.v len' == len
-      | _ -> False
-    end
-  ))
 
 #push-options "--z3rlimit 512 --z3cliopt smt.arith.nl=false"
 
