src/QUIC.Spec.Public.fsti
@@ -1,0 +1,127 @@
+module QUIC.Spec.Public
+
+module LP = LowParse.Spec.Base
+module U32 = FStar.UInt32
+module U62 = QUIC.UInt62
+module U64 = FStar.UInt64
+module U8 = FStar.UInt8
+module LPB = LowParse.BitFields
+module FB = FStar.Bytes
+
+inline_for_extraction
+let short_dcid_len_t = (short_dcid_len: U32.t { U32.v short_dcid_len <= 20 })
+
+inline_for_extraction
+noextract
+let token_max_len = 16383 // arbitrary bound
+
+inline_for_extraction
+let vlbytes (min: nat) (max: nat) =
+  (x: FB.bytes { min <= FB.length x /\ FB.length x <= max })
+
+inline_for_extraction
+noextract
+let bitfield
+  (sz: nat { sz <= 8 })
+: Tot eqtype
+= (x: U8.t { U8.v x < pow2 sz })
+
+inline_for_extraction
+let payload_and_pn_length_t : Type0 =
+  (payload_and_pn_length: U62.t { U64.v payload_and_pn_length >= 20 })
+
+noeq
+type long_header_specifics =
+| PInitial:
+  (token: vlbytes 0 token_max_len) -> // arbitrary bound
+  (payload_and_pn_length: payload_and_pn_length_t) ->
+  long_header_specifics
+| PZeroRTT:
+  (payload_and_pn_length: payload_and_pn_length_t) ->
+  long_header_specifics
+| PHandshake:
+  (payload_and_pn_length: payload_and_pn_length_t) ->
+  long_header_specifics
+| PRetry:
+  (odcid: vlbytes 0 20) -> // TODO: change bounds to drop instead of rejecting as invalid
+  long_header_specifics
+
+noeq
+type header =
+| PLong:
+  (protected_bits: bitfield 4) ->
+  (version: U32.t) ->
+  (dcid: vlbytes 0 20) ->
+  (scid: vlbytes 0 20) ->
+  (spec: long_header_specifics) ->
+  header
+| PShort:
+  (protected_bits: bitfield 5) ->
+  (spin: bool) ->
+  (dcid: vlbytes 0 20) ->
+  header
+
+let dcid_len (h: header) : Tot nat =
+  match h with
+  | PLong _ _ dcid _ _ -> FB.length dcid
+  | PShort _ _ dcid -> FB.length dcid
+
+let short_dcid_len_prop
+  (short_dcid_len: short_dcid_len_t)
+  (h: header)
+: GTot Type0
+= (PShort? h ==> dcid_len h == U32.v short_dcid_len)
+
+unfold
+let parse_header_prop
+  (short_dcid_len: short_dcid_len_t)
+  (m: header)
+: GTot Type0
+= short_dcid_len_prop short_dcid_len m
+
+inline_for_extraction
+type header'
+  (short_dcid_len: short_dcid_len_t)
+= (m: header { parse_header_prop short_dcid_len m })
+
+inline_for_extraction
+noextract
+val parse_header_kind'
+  (short_dcid_len: short_dcid_len_t)
+: Tot LP.parser_kind
+
+val parse_header
+  (short_dcid_len: short_dcid_len_t)
+: Tot (LP.parser (parse_header_kind' short_dcid_len) (header' short_dcid_len))
+
+val serialize_header
+  (short_dcid_len: short_dcid_len_t)
+: Tot (LP.serializer (parse_header short_dcid_len))
+
+
+(* Mutating the protected bits *)
+
+let get_protected_bits
+  (h: header)
+: Tot (bitfield (if PShort? h then 5 else 4))
+= match h with
+  | PShort pb spin dcid -> pb
+  | PLong pb version dcid scid spec -> pb
+
+let set_protected_bits
+  (h: header)
+  (new_pb: bitfield (if PShort? h then 5 else 4))
+: Tot header
+= match h with
+  | PShort _ spin dcid -> PShort new_pb spin dcid
+  | PLong _ version dcid scid spec -> PLong new_pb version dcid scid spec
+
+val serialize_set_protected_bits
+  (short_dcid_len: short_dcid_len_t)
+  (h: header' short_dcid_len)
+  (new_pb: bitfield (if PShort? h then 5 else 4))
+: Lemma
+  (let sq = LP.serialize (serialize_header short_dcid_len) h in
+  Seq.length sq > 0 /\
+  LP.serialize (serialize_header short_dcid_len) (set_protected_bits h new_pb) `Seq.equal`
+    (LPB.uint8.LPB.set_bitfield (Seq.head sq) 0 (if PShort? h then 5 else 4) new_pb `Seq.cons` Seq.tail sq))
